test

src/lib/inst/Kuiper.MatMul.Tiled.SHMem.fst
@@ -9,9 +9,9 @@ module M4 = Kuiper.Matrix4
 module Tiled = Kuiper.MatMul.Tiled
 friend Kuiper.MatMul.Tiled
 
-let inst = 
+let inst_gpu = 
    P.matmul_gpu 32sz
-   #f32 #_ #32sz #32sz #32sz
+   #u64 #_ #32sz #32sz #32sz
    (R.row_major 1024 1024)
    (R.row_major 1024 1024)
    (R.row_major 1024 1024)
@@ -24,3 +24,39 @@ let inst =
    #(Tiled.clayout4_from_clayout #32sz #32sz 32sz
      #(R.row_major 1024 1024)
      (R.crepr_row_major.map 1024sz 1024sz))
+
+fn matmul
+  (a : vec u64)
+  (b : vec u64)
+  (#sa : erased (seq u64){ len sa == 1024 * 1024 })
+  (#sb : erased (seq u64){ len sb == 1024 * 1024 })
+  preserves
+   cpu ** (a |-> sa) ** (b |-> sb)
+  requires
+   pure (three_fits 1024 1024 1024) **
+   pure (1024 * 1024 <= max_blocks)
+  returns
+    c : vec u64
+  ensures
+   exists* sc. c |-> sc
+{
+  let gA = M4.gpu_matrix_alloc0 #u64 32sz 32sz 32sz 32sz (R.row_major 1024 1024);
+  let gB = M4.gpu_matrix_alloc0 #u64 32sz 32sz 32sz 32sz (R.row_major 1024 1024);
+  let gC = M4.gpu_matrix_alloc0 #u64 32sz 32sz 32sz 32sz (R.row_major 1024 1024);
+
+  M4.gpu_matrix_from_array #u64 #_ #32sz #32sz #32sz #32sz gA a;
+  M4.gpu_matrix_from_array #u64 #_ #32sz #32sz #32sz #32sz gB b;
+
+  with vc. assert gC |-> vc;
+
+  inst_gpu gA gB gC;
+
+  let c = Pulse.Lib.Vec.alloc #u64 zero (1024sz *^ 1024sz);
+  M4.gpu_matrix_to_array #_ #_ #32sz #32sz #32sz #32sz c gC;
+
+  M4.gpu_matrix_free gA;
+  M4.gpu_matrix_free gB;
+  M4.gpu_matrix_free gC;
+
+  c
+}
